cache store invariant about history

new/proof/go_etcd_io/etcd/cache/v3.v
@@ -37,19 +37,34 @@ Local Set Default Proof Using "W".
    away. *)
 Axiom own_ringBuffer :
   ∀ (r : loc) [T'] `[!ZeroVal T'] `[!TypedPointsto (Σ:=Σ) T'] [V]
-    (is_item : T' → V → iProp Σ) (item_rev : V → w64) (buf : list V), iProp Σ.
+    (is_item : T' → V → iProp Σ) (rev_item : V → w64) (buf : list V), iProp Σ.
+
+Context [T'] `[!ZeroVal T'] `[!TypedPointsto (Σ:=Σ) T'] [V] `[!IntoValTyped T' T]
+    (is_item : T' → V → iProp Σ) (rev_item : V → w64).
 
 Axiom wp_ringBuffer__PeekOldest :
-  ∀ (r : loc) [T'] `[!ZeroVal T'] `[!TypedPointsto (Σ:=Σ) T'] `[!IntoValTyped T' T] [V]
-    (is_item : T' → V → iProp Σ) (item_rev : V → w64) (buf : list V),
+  ∀ r buf,
   {{{ is_pkg_init cache ∗
-      own_ringBuffer r is_item item_rev buf }}}
+      own_ringBuffer r is_item rev_item buf }}}
     r @! (go.PointerType (cache.ringBuffer T)) @! "PeekOldest" #()
-  {{{ RET #(last (item_rev <$> buf) (W64 0));
-      own_ringBuffer r is_item item_rev buf }}}.
+  {{{ RET #(last (rev_item <$> buf) (W64 0));
+      own_ringBuffer r is_item rev_item buf }}}.
+
+Axiom wp_ringBuffer__DescendLessOrEqual_once :
+  ∀ (pivot : w64) (iter : func.t) r buf,
+  {{{ is_pkg_init cache ∗
+      own_ringBuffer r is_item rev_item buf ∗
+      (∀ Ψ i item,
+         ⌜ buf !! i = Some item ⌝ ∗
+         ⌜ sint.Z (rev_item item) ≤ sint.Z pivot ⌝ ∗
+         ⌜ Forall (λ itm, sint.Z pivot < sint.Z (rev_item itm)) (drop i buf) ⌝ -∗
+         Ψ #false -∗
+         WP #iter #(rev_item item) #item {{ Ψ }})
+  }}}
+    r @! (go.PointerType (cache.ringBuffer T)) @! "DescendLessOrEqual " #pivot #iter
+  {{{ RET #(); own_ringBuffer r is_item rev_item buf }}}.
 
 End ring_buffer.
-
 
 Section store.
 Context `{hG: heapGS Σ, !ffi_semantics _ _}.
@@ -57,18 +72,43 @@ Context {sem : go.Semantics} {package_sem : cache.Assumptions}.
 Collection W := sem + package_sem.
 Local Set Default Proof Using "W".
 
+(* for BTree *)
 Definition kvItem : Type := (go_string + KeyValue.t).
 Axiom is_kvItem : loc → kvItem → iProp Σ.
 Axiom less_kvItem : kvItem → kvItem → Prop.
 
+(* for ringbuffer *)
+Definition snap : Type := (w64 * list KeyValue.t).
+Axiom is_snapshotItem : loc → snap → iProp Σ.
+Definition rev_snapshotItem : snap → w64 := fst.
+
+Axiom is_etcd_kvs :
+  ∀ (revision : w64) (prefix : go_string) (key_values : gmap go_string KeyValue.t), iProp Σ.
+Axiom is_etcd_kvmap_pers : ∀ revision prefix key_values,
+  Persistent (is_etcd_kvs revision prefix key_values).
+Global Existing Instance is_etcd_kvmap_pers.
+
+Definition ordered_kvs_to_map (kvs : list KeyValue.t) : gmap go_string KeyValue.t :=
+  list_to_map ((λ kv, (kv.(KeyValue.key), kv)) <$> kvs).
+
 (* Cannot be persistent because of RWMutex. *)
-Definition own_store (s : loc) : iProp Σ :=
+Definition own_store (s : loc) (prefix : go_string) : iProp Σ :=
   "Hmu" ∷ own_RWMutex (s.[cache.store.t, "mu"])
     (λ q,
-       ∃ snapshot kvs_ordered,
+       ∃ snapshot kvs_ordered history,
        "latest" ∷ s.[cache.store.t, "latest"] ↦ snapshot ∗
        "latest_tree" ∷ (own_BTree (snapshot.(cache.snapshot.tree'))
-                          is_kvItem less_kvItem kvs_ordered (DfracOwn q)) ∗
+                          is_kvItem less_kvItem (inr <$> kvs_ordered) (DfracOwn q)) ∗
+       "history" ∷ (own_ringBuffer (s.[cache.store.t, "history"])
+                       is_snapshotItem rev_snapshotItem history) ∗
+       "#Hhistory" ∷ (
+           let history' := history ++ [(snapshot.(cache.snapshot.rev'), kvs_ordered)] in
+           ∀ revision i prev next,
+             ⌜ (history' !! i) = Some prev ∧
+               (history' !! (S i)) = Some next ∧
+               (sint.Z prev.1 ≤ sint.Z revision < sint.Z next.1) ⌝ →
+             is_etcd_kvs revision prefix (ordered_kvs_to_map prev.2)
+         ) ∗
        (* latest.rev seems like it must be monotonic, since linearizable Get
           relies on checking lower bound before reading. *)
        True
@@ -81,8 +121,8 @@ Definition is_snapshot (snap_ptr : loc) (kvs : gmap go_string KeyValue.t) : iPro
 Definition is_etcd_state (rev : w64) (kvs : gmap go_string KeyValue.t) : iProp Σ :=
   True.
 
-Lemma wp_store__getSnapshot s (rev : w64) :
-  {{{ is_pkg_init cache ∗ "Hs" ∷ own_store s }}}
+Lemma wp_store__getSnapshot s (rev : w64) prefix :
+  {{{ is_pkg_init cache ∗ "Hs" ∷ own_store s prefix }}}
     s @! (go.PointerType cache.store) @! "getSnapshot" #rev
   {{{ snap_ptr snap_rev err, RET (#snap_ptr, #snap_rev, #err);
       match err with
@@ -110,6 +150,13 @@ Proof.
   wp_if_destruct.
   { (* TODO: rpctypes global error variable. *) admit. }
   (* TODO: spec for peekoldest *)
+  wp_apply (wp_ringBuffer__PeekOldest with "[$Hhistory_inv]").
+  iIntros "Hhistory_inv". wp_auto.
+  wp_if_destruct.
+  { (* TODO: global rpctypes.ErrCompacted *) admit. }
+  (* FIXME: the next line is buggy. *)
+  wp_auto.
+
 Admitted.
 
 End store.
